

MATH 352B- HW2 (Raphael F. Loy - U30156477)

① Consider the i-b value problem: $\frac{\partial u}{\partial t} = D \frac{\partial^2 u}{\partial x^2}$, $0 < x < \pi$, $t > 0$; $u(x, 0) = f(x)$; $u(0, t) = u(\pi, t) = 0$

a) Now, by separation of variables, solve $\frac{\partial u}{\partial t} = D \frac{\partial^2 u}{\partial x^2} + a \frac{\partial u}{\partial x}$

$$\Rightarrow u(x, t) = X(x)T(t) \rightarrow \frac{\partial}{\partial t}(X \cdot T) = D \frac{\partial^2}{\partial x^2}(X \cdot T) + a \frac{\partial}{\partial x}(X \cdot T)$$

$$\rightarrow XT' = DX''T + aXT' \xrightarrow[\text{by } DX'T]{\text{dividing}} \frac{T'}{DT} = \frac{X''}{Xa} + \frac{X'}{XD} = -\lambda$$

\Rightarrow The ODE's we obtain are: $T' = -\lambda DaT$ and $DX'' + aX' + \lambda X = 0$

b) Back to the original PDE, for the eigenvalue problem $X'' + \lambda X = 0$, $X(0) = X(\pi) = 0$, we need to find all λ that give a non-trivial solution $X(x)$. Show that for $\lambda \leq 0$, the only solution is $X(x) = 0$.

\Rightarrow Case $\lambda = 0$: $X'' = 0 \xrightarrow{\text{gen. sol.}} X(x) = ax + b$

$$\begin{aligned} X(0) &= a \cdot 0 + b = 0 \Rightarrow b = 0 \\ X(\pi) &= a \cdot \pi = 0 \Rightarrow a = 0 \end{aligned} \} X(x) = 0x + 0 = 0$$

Case $\lambda < 0$: let's write $\lambda = -\gamma^2$. In this case we have $\begin{cases} X'' - \gamma^2 X = 0 \\ X(0) = X(\pi) = 0 \end{cases}$

In this case, the general solution is given by $X(x) = a \cosh(\gamma x) + b \sinh(\gamma x)$

$$X(0) = a \cosh(0) + b \sinh(0) = a \left(\frac{e^0 + e^{-0}}{2} \right) + b \left(\frac{e^0 - e^{-0}}{2} \right) = a \cdot 1 + b \cdot 0 = a = 0$$

$$X(\pi) = b \sinh(\gamma \pi) = b \left(\frac{e^{\gamma \pi} - e^{-\gamma \pi}}{2} \right) = b \left(\frac{1 - e^{-2\gamma \pi}}{2e^{-\gamma \pi}} \right) = 0 \Rightarrow b = 0$$

\Rightarrow We have shown that for $\lambda \leq 0$, the only solution is $X(x) = 0$ $\hookrightarrow X(x) = 0 \cosh(\gamma x) + 0 \sinh(\gamma x) = 0$

② Consider the i-b value problem, defined on the interval $x \in [a, b]$: $\frac{\partial u}{\partial t} = D \frac{\partial^2 u}{\partial x^2}$, $a < x < b$, $t > 0$

Reduce this problem to the original by a change of variables. $u(x, 0) = \tilde{f}(x)$
 $u(a, t) = u(b, t) = 0$

\Rightarrow Using the hint, let $\xi = \pi \frac{(x-a)}{(b-a)}$. When $x = a$, $\xi = \pi \frac{(a-a)}{(b-a)} = 0$. Therefore, for $a < x < b$, $0 < \xi < \pi$
When $x = b$, $\xi = \pi \frac{(b-a)}{(b-a)} = \pi$

Now, to find $\frac{\partial^2 u}{\partial x^2}$ in terms of ξ : $\frac{\partial u}{\partial x} = \frac{du}{d\xi} \cdot \frac{d\xi}{dx}$; $\frac{\partial^2 u}{\partial x^2} = \frac{d}{d\xi} \left(\frac{du}{d\xi} \cdot \frac{d\xi}{dx} \right) \cdot \frac{d\xi}{dx}$, where $\frac{d\xi}{dx} =$

$$= \frac{\partial}{\partial x} \left(\pi \frac{(x-a)}{(b-a)} \right) = \frac{\pi}{b-a} \frac{\partial}{\partial x} (x-a) = \frac{\pi}{b-a} \left(\frac{\partial x}{\partial x} \frac{\partial}{\partial x} \right) = \frac{\pi}{b-a}$$

$$\text{Now we have } \frac{\partial u}{\partial t} = \tilde{D} \left(\frac{d}{d\xi} \left(\frac{\partial u}{\partial \xi} \cdot \frac{\pi}{b-a} \right) \frac{\pi}{b-a} \right) \rightarrow \int \frac{d}{d\xi} \left(\frac{\partial u}{\partial \xi} \cdot \frac{\pi}{b-a} \right) d\xi = \frac{\partial u}{\partial \xi} \cdot \frac{\pi}{b-a} + C$$

$$u(\xi, 0) = \tilde{f}(\xi); \quad u(0, t) = u(\pi, t) = 0$$

$$\Rightarrow \int \frac{\partial u}{\partial t} dt = \tilde{D} \left(\frac{\pi}{b-a} \right)^2 \int \frac{d^2}{d\xi^2} u d\xi \rightarrow u(\xi, t) = \underbrace{\left(\tilde{D} \left(\frac{\pi}{b-a} \right)^2 \right)}_{\text{"D"}} \int \frac{d^2}{d\xi^2} u d\xi + C$$

Reducing to the original: $\frac{\partial u}{\partial t} = \left[\tilde{D} \left(\frac{\pi}{b-a} \right)^2 \right] \frac{\partial^2 u}{\partial \xi^2}$, $0 < \xi < \pi$; $u(\xi, 0) = \tilde{f}(\xi) = f(\xi)$; $u(0, t) = u(\pi, t) = 0$.

③ Consider the reaction-diffusion eq. on $x \in (-\infty, \infty)$: $\frac{\partial u}{\partial t} = D \frac{\partial^2 u}{\partial x^2} + ru$, $t > 0$.

a) Show that the following function satisfies the PDE: $u(x, t) = \frac{u_0}{2(\pi Dt)^{1/2}} \exp \left\{ rt - \frac{x^2}{4Dt} \right\}$

→ Starting with $r=0$ to verify, we can use Fourier Transform:

$$u_t = Du_{xx} \rightarrow \hat{u}_t = D\hat{u}_{xx} \rightarrow \hat{u}_t = D(-is)^2 \hat{u} = -Ds^2 \hat{u} \rightarrow \hat{u}(s, t) = C e^{-Ds^2 t}$$

OBS: $y' = ay \rightarrow y = C e^{at}$

OBS: $C = \hat{u}(s, 0) = \hat{u}(x, 0) = \hat{f}(x) = \hat{f}(s)$

OBS: $\int e^{-ax^2+bx} dx = e^{b^2/4a} \sqrt{\frac{\pi}{a}}$

To get $u(x, t)$: $\hat{u}(s, t) = \frac{1}{2\pi} \int_{-\infty}^{\infty} C e^{-Ds^2 t} e^{-isx} ds = u(x, t)$

$$\Rightarrow \frac{1}{2\pi} \int_{-\infty}^{\infty} e^{-Ds^2 t} e^{-isx} ds = \frac{1}{2\pi} \int_{-\infty}^{\infty} e^{-Ds^2 t - isx} ds \rightarrow a = Dt, b = -ix$$

$$\Rightarrow \frac{1}{2\pi} e^{(-ix)^2/4Dt} \sqrt{\frac{\pi}{Dt}} = \frac{1}{\sqrt{4\pi Dt}} e^{-x^2/4Dt} = u(x, t)$$

Now, for $r > 0$: $u_t = Du_{xx} + ru \rightarrow \hat{u}_t = D\hat{u}_{xx} + r\hat{u} = D(-is)^2 \hat{u} + r\hat{u} = (-Ds^2 + r)\hat{u}$

$$\Rightarrow \hat{u}(s, t) = C e^{(-Ds^2 + r)t} \rightarrow \hat{u}(s, t) = \frac{1}{2\pi} \int_{-\infty}^{\infty} C e^{(-Ds^2 + r)t} e^{-isx} ds = u(x, t)$$

$$\Rightarrow \frac{1}{2\pi} \int_{-\infty}^{\infty} e^{(-Ds^2 + r)t} e^{-isx} ds = \frac{1}{2\pi} \int_{-\infty}^{\infty} e^{(-Ds^2 + r)t - isx} ds \rightarrow a = Dt, b = -ix \rightarrow \frac{1}{2\pi} e^{rt + (-ix)^2/4Dt} \sqrt{\frac{\pi}{Dt}}$$

$$= \frac{1}{\sqrt{4\pi Dt}} e^{rt - x^2/4Dt} \approx \text{what about the } u_0?$$

③ b) Consider the level set $u(x, t) = U$ (const.). Show that on this contour, the ratio $\frac{x}{t}$ satisfies $\frac{x}{t} = \pm \left[4rD - \frac{2D}{t} \ln t - \frac{4D}{t} \ln \left(\frac{U}{u_0} \right) \right]^{\frac{1}{2}}$

\Rightarrow From a), let's use that $u(x, t) = \frac{u_0}{2\sqrt{\pi Dt}} e^{rt - \frac{x^2}{4Dt}} = U$. Therefore:

$$e^{rt - \frac{x^2}{4Dt}} = \frac{U}{u_0} \cdot 2\sqrt{\pi Dt} \Rightarrow rt - \frac{x^2}{4Dt} = \ln \frac{U}{u_0} \cdot 2\sqrt{\pi Dt} \Rightarrow \frac{x^2}{4Dt} = rt - \ln \frac{U}{u_0} 2\sqrt{\pi Dt}$$

$$\Rightarrow x^2 = 4Dt(rt - \ln \frac{U}{u_0} 2\sqrt{\pi Dt}) \Rightarrow x = \pm \sqrt{4Dt(rt - \ln \frac{U}{u_0} 2\sqrt{\pi Dt})}$$

$$\Rightarrow \frac{x}{t} = \pm \sqrt{\frac{4Dt(rt - \ln \frac{U}{u_0} 2\sqrt{\pi Dt})}{t^2}} = \pm \sqrt{\frac{4Dr t^2 - 4Dt \ln \sqrt{t} - 4Dt \ln \frac{U}{u_0} 2\sqrt{\pi}}{t^2}}$$

$$\Rightarrow \frac{x}{t} = \pm \sqrt{\frac{4Dr t^2 - 4Dt \left(\frac{1}{2} \right) \ln t - 4Dt \frac{U}{u_0} 2\sqrt{\pi}}{t^2}} = \pm \sqrt{4Dr - \frac{2D}{t} \ln t - \frac{4D}{t} (2\sqrt{\pi} \frac{U}{u_0})}$$

c) Show that as $t \rightarrow \infty$, one can approximate the above by $\frac{x}{t} = \pm 2\sqrt{rD}$

$$\Rightarrow \text{As } t \rightarrow \infty, \lim_{t \rightarrow \infty} -\frac{2D}{t} \ln t \approx -2D \lim_{t \rightarrow \infty} \frac{\ln t}{t} \approx -2D \lim_{t \rightarrow \infty} \frac{\frac{1}{t}}{\frac{1}{t}} = \frac{1}{t} = 0. \text{ As}$$

U, D and u_0 are all constants, the second \ln also goes to 0 as $t \rightarrow \infty$,
therefore we can approximate the above to $\frac{x}{t} = \pm \sqrt{4Dr} = 2\sqrt{rD}$.

③ a) (Cont.) We have verified that, from the PDE, $u(x,t)$ can be found to be $u(x,t) = \frac{1}{2(\pi Dt)^{1/2}} \exp\left\{rt - \frac{x^2}{4Dt}\right\}$. Now, we must do the other way around, and confirm that the function satisfies the PDE.

$\Rightarrow \frac{u_0}{2(\pi Dt)^{1/2}} \exp\left\{rt - \frac{x^2}{4Dt}\right\}$. Knowing $e^{b^2/4a} \sqrt{\frac{\pi}{a}} = \int_{-\infty}^{\infty} e^{-ax^2+bx} dx$, we write $a=Dt$, $b=-ix$, and get

$$\Rightarrow \frac{u_0}{2\pi} \exp\left\{rt + \frac{(-ix)^2}{4Dt}\right\} \sqrt{\frac{\pi}{Dt}} \Rightarrow \frac{1}{2\pi} \int_{-\infty}^{\infty} e^{(-Ds^2+r)t - isx} ds, \text{ where } \hat{f}(s) = \hat{f}(x) = u(x,0)$$

$$\Rightarrow \frac{1}{2\pi} \int_{-\infty}^{\infty} u_0 e^{(-Ds^2+r)t} e^{-isx} ds = \hat{u}(s,t) \Rightarrow \hat{u}(s,t) = u_0 e^{(-Ds^2+r)t}$$

$$\Rightarrow (-Ds^2+r)\hat{u} = D(-is)^2\hat{u} + r\hat{u} = D\hat{u}_{xx} + r\hat{u} = \hat{u}_t$$

$$\Rightarrow Du_{xx} + ru = u_t$$

$$D \frac{\partial^2 u}{\partial x^2} + ru = \frac{\partial u}{\partial t} //$$